coq_monadic/era_inv.v
@@ -30,6 +30,31 @@ Proof.
   exists A. by exists m.
 Qed.
 
+Lemma era_it_form Γ Δ m A : Γ ; Δ ⊢ m ~ It : A -> m = It.
+Proof. move e:(It)=>x er. elim: er e=>//{Γ Δ m x A}. Qed.
+
+Lemma era_num_form Γ Δ m n A : Γ ; Δ ⊢ m ~ Num n : A -> m = Num n.
+Proof. move e:(Num n)=>x er. elim: er n e=>//{Γ Δ m x A}. Qed.
+
+Lemma era_rand_form Γ Δ m A : Γ ; Δ ⊢ m ~ Rand : A -> m = Rand.
+Proof. move e:(Rand)=>x er. elim: er e=>//{Γ Δ m x A}. Qed.
+
+Lemma era_randit_form Γ Δ m A :
+  Γ ; Δ ⊢ m ~ App Rand It : A -> m = App Rand It.
+Proof.
+  move e:(App Rand It)=>x er. elim: er e=>//{Γ Δ m x A}.
+  move=>Γ Δ1 Δ2 Δ A B m m' n n' s mrg erm ihm ern ihn[e1 e2]. subst.
+  have->:=era_rand_form erm.
+  have->//:=era_it_form ern.
+Qed.
+
+Lemma era_return_form Γ Δ m n A :
+  Γ ; Δ ⊢ m ~ Return n : A -> exists n, m = Return n.
+Proof.
+  move e:(Return n)=>x er. elim: er n e=>//{Γ Δ m x A}.
+  move=>Γ Δ m m' A erm ihm n[e]. subst. exists m=>//.
+Qed.
+
 Lemma era_box_form Γ Δ m A : ~Γ ; Δ ⊢ m ~ Box : A.
 Proof. move e:(Box)=>m' ty. elim: ty e=>//{Γ Δ m m' A}. Qed.
 
@@ -103,4 +128,20 @@ Proof with eauto.
   move=>ty.
   have[t/sta_pi1_inv[r[tyB _]]]:=dyn_valid (era_dyn_type ty).
   apply: era_lam1_invX...
+Qed.
+
+Lemma era_return_inv Γ Δ m m' B :
+  Γ ; Δ ⊢ Return m ~ Return m' : B ->
+  exists A, Γ ; Δ ⊢ m ~ m' : A /\ B === IO A.
+Proof with eauto.
+  move e1:(Return m)=>n.
+  move e2:(Return m')=>n' tyR.
+  elim: tyR m m' e1 e2=>//{Γ Δ n n' B}.
+  { move=>Γ Δ m m' A erm ihm m0 m'0[e1][e2]; subst. exists A... }
+  { move=>Γ Δ A B m m' s eq1 erm ihm tyB m0 m'0 e1 e2; subst.
+    have[A0[erm0 eq2]]:=ihm _ _ erefl erefl.
+    exists A0. split...
+    apply: conv_trans.
+    apply: conv_sym...
+    exact: eq2. }
 Qed.
