coq_monadic/era_prog.v
@@ -22,6 +22,21 @@ Proof with eauto.
   exists m'...
 Qed.
 
+Lemma era_rand_canonical Γ Δ A m :
+  Γ ; Δ ⊢ Rand ~ m : A -> m = Rand.
+Proof. move e:(Rand)=>x ty. elim: ty e=>//{Γ Δ x m A}. Qed.
+
+Lemma era_it_canonical Γ Δ A m :
+  Γ ; Δ ⊢ It ~ m : A -> m = It.
+Proof. move e:(It)=>x ty. elim: ty e=>//{Γ Δ x m A}. Qed.
+
+Lemma era_return_canonical Γ Δ A m n :
+  Γ ; Δ ⊢ Return m ~ n : A -> exists m, n = Return m.
+Proof.
+  move e:(Return m)=>x ty. elim: ty m e=>//{Γ Δ x n A}.
+  move=>Γ Δ m m' A erm ihm m0[e]; subst. exists m'=>//.
+Qed.
+
 Lemma era_prog m m' A :
   nil ; nil ⊢ m ~ m' : A -> (exists n', m' ~>> n') \/ dyn_val m'.
 Proof with eauto using dyn_step, dyn_val.
@@ -35,8 +50,7 @@ Proof with eauto using dyn_step, dyn_val.
   { move=>Γ Δ A B m m' n s erm ihm tyn e1 e2; subst.
     have[[x st]|vl]:=ihm erefl erefl.
     { left. exists (App x Box)... }
-    { left.
-      have{}vl:=era_dyn_val vl erm.
+    { left. have{}vl:=era_dyn_val erm vl.
       have tym:=era_dyn_type erm.
       have[A0[n0 e]]:=dyn_pi0_canonical tym (convR _ _) vl. subst.
       have[m0 e]:=era_lam0_canonical erm. subst.
@@ -44,12 +58,62 @@ Proof with eauto using dyn_step, dyn_val.
   { move=>Γ Δ1 Δ2 Δ A B m m' n n' s mrg erm ihm ern ihn e1 e2; subst.
     inv mrg. have[[mx st1]|vlm]:=ihm erefl erefl.
     { left. exists (App mx n')... }
-    { left. have[[nx st2]|vln]:=ihn erefl erefl.
-      exists (App m' nx)...
-      have{}vlm:=era_dyn_val vlm erm.
-      have tym:=era_dyn_type erm.
-      have[A0[n0 e]]:=dyn_pi1_canonical tym (convR _ _) vlm. subst.
-      have[m0 e]:=era_lam1_canonical erm. subst.
-      exists (m0.[n'/])... } }
+    { have[[nx st2]|vln']:=ihn erefl erefl.
+      { left. exists (App m' nx)... }
+      { have{}vlm:=era_dyn_val erm vlm.
+        have tym:=era_dyn_type erm.
+        have[e|[A0[n0 e]]]:=dyn_pi1_canonical tym (convR _ _) vlm. subst.
+        { have e:=era_rand_canonical erm. subst.
+          have[/pi1_inj[eq1[eq2 e]] _]:=dyn_rand_inv (era_dyn_type erm). subst.
+          have{}ern:=era_conv eq1 ern (sta_unit sta_wf_nil).
+          have vln:=era_dyn_val ern vln'.
+          have e:=dyn_unit_canonical (era_dyn_type ern) (convR _ _) vln. subst.
+          have e:=era_it_canonical ern. subst. right... }
+        { subst. have[m1 e]:=era_lam1_canonical erm. subst.
+          left. exists m1.[n'/]... } } } }
+  { move=>Γ Δ k wf e1 e2; subst. right... }
+  { move=>Γ Δ n k wf e1 e2; subst. right... }
+  { move=>Γ Δ k wf e1 e2; subst. right... }
+  { move=>Γ Δ m m' A erm ihm e1 e2; subst.
+    have[[n' st]|vlm']:=ihm erefl erefl.
+    { left. exists (Return n')... }
+    { right... } }
+  { move=>Γ Δ1 Δ2 Δ m m' n n' A B s t mrg tyB erm ihm ern ihn e1 e2; subst. inv mrg.
+    have[[m'0 st]|vlm']:=ihm erefl erefl.
+    { left. exists (LetIn m'0 n')... }
+    { right... } }
   { move=>Γ Δ A B m m' s eq tym ihm tyB e1 e2; subst... }
+Qed.
+
+Lemma era_mprog m m' A R :
+  nil ; nil ⊢ m ~ m' : A -> (exists T n', R ; m' ~>> T ; n') \/ dyn_mval m'.
+Proof with eauto using dyn_mstep, dyn_step, dyn_mval.
+  move e1:(nil)=>Γ.
+  move e2:(nil)=>Δ ty. elim: ty e1 e2 R=>{Γ Δ m m' A}.
+  { move=>Γ Δ x s A wf shs dhs e1 e2 R. subst. inv shs. }
+  { move=>Γ Δ A B m m' s k erm ihm e1 e2 R. subst. right... }
+  { move=>Γ Δ A B m m' s t k erm ihm e1 e2 R. subst. right... }
+  { move=>Γ Δ A B m m' n s erm ihm tyn e1 e2 R. subst. left.
+    have[[x st]|vl]:=era_prog (era_app0 erm tyn).
+    { exists R. exists x... }
+    { inv vl. } }
+  { move=>Γ Δ1 Δ2 Δ A B m m' n n' s mrg erm ihm ern ihn e1 e2 R. subst. left.
+    have[[x st]|vl]:=era_prog (era_app1 mrg erm ern).
+    { exists R. exists x... }
+    { inv vl. exists R.+1. exists (Return (Num R))... } }
+  { move=>Γ Δ k wf e1 e2 R. subst. right... }
+  { move=>Γ Δ n k wf e1 e2 R. subst. right... }
+  { move=>Γ Δ k wf e1 e2 R. subst. right... }
+  { move=>Γ Δ m m' A erm ihm e1 e2 R. subst.
+    have[[n' st]|vl]:=era_prog erm.
+    { left. exists R. exists (Return n')... }
+    { right... } }
+  { move=>Γ Δ1 Δ2 Δ m m' n n' A B s t mrg tyB erm ihm ern ihn e1 e2 R. subst. inv mrg.
+    left. have[[T[m0 st]]|vlm']:=ihm erefl erefl R.
+    { exists T. exists (LetIn m0 n')... }
+    { have vlm:=era_dyn_mval erm vlm'.
+      have[n0 e]:=dyn_io_canonical (era_dyn_type erm) (convR _ _) vlm. subst.
+      have[m e]:=era_return_canonical erm. subst. inv vlm'.
+      exists R. exists n'.[m/]... } }
+  { move=>Γ Δ A B m m' s eq1 erm ihm tyB e1 e2 R. subst... }
 Qed.
