coq_monadic/era_sr.v
@@ -7,12 +7,27 @@ Unset Strict Implicit.
 Unset Printing Implicit Defensive.
 
 Lemma era_dyn_val Γ Δ m m' A :
-  dyn_val m' -> Γ ; Δ ⊢ m ~ m' : A -> dyn_val m.
+  Γ ; Δ ⊢ m ~ m' : A -> dyn_val m' -> dyn_val m.
 Proof with eauto using dyn_val.
-  move=>vl. inv vl.
-  { move=>/era_var_form[x' e]; subst... }
-  { move=>/era_lam0_form[A'[m' e]]; subst... }
-  { move=>/era_lam1_form[A'[m' e]]; subst... }
+  move=>ty. elim: ty=>{Γ Δ m m' A}...
+  { move=>Γ Δ A B m m' n s erm ih tyn vl. inv vl. }
+  { move=>Γ Δ1 Δ2 Δ A B m m' n n' s mrg erm ihm ern ihn vl. inv vl.
+    have->:=era_rand_form erm.
+    have->:=era_it_form ern.
+    constructor... }
+  { move=>Γ Δ m m' A erm ihm vl. inv vl... }
+  { move=>Γ Δ1 Δ2 Δ m m' n n' A B s t mrg tyB erm ihm ern ihn vl. inv vl... }
+Qed.
+
+Lemma era_dyn_mval Γ Δ m m' A :
+  Γ ; Δ ⊢ m ~ m' : A -> dyn_mval m' -> dyn_mval m.
+Proof with eauto using dyn_mval, dyn_mval_val.
+  move=>ty. elim: ty=>{Γ Δ m m' A}...
+  { move=>Γ Δ A B m m' n s erm ih tyn vl. inv vl. }
+  { move=>Γ Δ1 Δ2 Δ A B m m' n n' s mrg erm ihm ern ihn vl. inv vl. }
+  { move=>Γ Δ m m' A erm ihm vl. inv vl.
+    have vl:=era_dyn_val erm H0... }
+  { move=>Γ Δ1 Δ2 Δ m m' n n' A B s t mrg tyB erm ihm ern ihn vl. inv vl... }
 Qed.
 
 Theorem era_sr Γ Δ m m' n' A :
@@ -60,6 +75,15 @@ Proof with eauto using dyn_step, era_type.
       apply: era_dyn_type...
       exact: H5.
       apply: era_dyn_val... } }
+  { move=>Γ Δ k wf n' st. inv st. }
+  { move=>Γ Δ n k wf n' st. inv st. }
+  { move=>Γ Δ k wf n' st. inv st. }
+  { move=>Γ Δ m m' A erm ihm n' st. inv st.
+    have[m0 st0 tym0]:=ihm _ H0.
+    exists (Return m0)... }
+  { move=>Γ Δ1 Δ2 Δ m m' n n' A B s t mrg tyB erm ihm ern ihn n'0 st. inv st.
+    have[m0 st0 tym0]:=ihm _ H2.
+    exists (LetIn m0 n)... }
   { move=>Γ Δ A B m m' s eq tym ihm tyB n' st.
     have[n st' tyn]:=ihm _ st.
     exists n... }
@@ -76,4 +100,59 @@ Proof with eauto.
   exists y...
   apply: star_trans...
   apply: star1...
+Qed.
+
+Theorem era_msr Γ Δ m m' n' A R T :
+  Γ ; Δ ⊢ m ~ m' : A -> R ; m' ~>> T ; n' ->
+  exists2 n, R ; m ~>> T ; n & Γ ; Δ ⊢ n ~ n' : A.
+Proof with eauto using
+  era_type, sta_step, dyn_step, dyn_mstep, dyn_wf, era_sr.
+  move=>ty. elim: ty n' R T=>{Γ Δ m m' A}.
+  { move=>Γ Δ x s A wf shs dhs n' R T st. inv st. inv H0. }
+  { move=>Γ Δ A B m m' s k erm ihm n' R T st. inv st. inv H0. }
+  { move=>Γ Δ A B m m' s t k erm ihm n' R T st. inv st. inv H0. }
+  { move=>Γ Δ A B m m' n s erm ihm tyn n' R T st. inv st.
+    have[x st ty]:=era_sr (era_app0 erm tyn) H0. exists x... }
+  { move=>Γ Δ1 Δ2 Δ A B m m' n n' s mrg erm ihm ern ihn n'0 R T st. inv st.
+    { have[x st ty]:=era_sr (era_app1 mrg erm ern) H0. exists x... }
+    { have wf1:=dyn_type_wf (era_dyn_type erm).
+      have wf2:=dyn_type_wf (era_dyn_type ern).
+      have e:=era_rand_form erm. subst.
+      have e:=era_it_form ern. subst.
+      have[t tyP]:=dyn_valid (era_dyn_type erm).
+      have[r[tyB/sort_inj e]]:=sta_pi1_inv tyP. subst.
+      have tyI:=dyn_sta_type (era_dyn_type ern).
+      have/=tyBI:=sta_subst tyB tyI.
+      have tyIO:=sta_io (sta_nat (dyn_sta_wf wf1)).
+      have[/pi1_inj[eq1[eq2 e]]k1]:=dyn_rand_inv (era_dyn_type erm). subst.
+      have[_ k2]:=dyn_it_inv (era_dyn_type ern).
+      pose proof (sta_conv_subst (It .: ids) eq2) as H. asimpl in H.
+      exists (Return (Num R))...
+      apply: era_conv.
+      apply: conv_sym...
+      apply: era_return.
+      apply: era_num...
+      apply: key_merge...
+      apply: dyn_wf_merge...
+      apply: tyBI. } }
+  { move=>Γ Δ k wf n' R T st. inv st. inv H0. }
+  { move=>Γ Δ n k wf n' R T st. inv st. inv H0. }
+  { move=>Γ Δ k wf n' R T st. inv st. inv H0. }
+  { move=>Γ Δ m m' A erm ihm n' R T st. inv st.
+    have[x st er]:=era_sr (era_return erm) H0. exists x... }
+  { move=>Γ Δ1 Δ2 Δ m m' n n' A B s t mrg tyB erm ihm ern ihn n'0 R T st. inv st.
+    { have[x st er]:=era_sr (era_letin mrg tyB erm ern) H0. exists x... }
+    { have[m0 st er]:=ihm _ _ _ H0. exists (LetIn m0 n)... }
+    { have wf:=dyn_type_wf (era_dyn_type ern). inv wf.
+      have[n0 e]:=era_return_form erm. subst.
+      have[A0[erv/io_inj eq]]:=era_return_inv erm.
+      have{}erv:=era_conv (conv_sym eq) erv H5.
+      have erv0:=era_dyn_val erv H0.
+      have k:=dyn_val_key (era_dyn_type erv) H5 erv0.
+      exists n.[n0/].
+      apply: dyn_mstep_letret...
+      have:=era_subst1 k (merge_sym mrg) ern erv.
+      autosubst. } }
+  { move=>Γ Δ A B m m' s eq erm ihm tyB n' R T st'.
+    have[n st er]:=ihm _ _ _ st'. exists n... }
 Qed.
